networkInvariantPrototypes/paxos/types.dfy
@@ -5,13 +5,15 @@ module Types {
 
   type LeaderId = nat
   type AcceptorId = nat
+  type LearnerId = nat
   type Value
   datatype ValBal = VB(v:Value, b:LeaderId)
 
   datatype Message = Prepare(bal:LeaderId)
-                  | Promise(bal:LeaderId, acc:AcceptorId,vbOpt:Option<ValBal>)  //valbal is the value-ballot pair with which the value was accepted
+                  | Promise(bal:LeaderId, acc:AcceptorId, vbOpt:Option<ValBal>)  //valbal is the value-ballot pair with which the value was accepted
                   | Propose(bal:LeaderId, val:Value)
-                  | Accept(bal:LeaderId, val:Value)
+                  | Accept(vb:ValBal, acc:AcceptorId)
+                  | Learn(val:Value)
 
   datatype MessageOps = MessageOps(recv:Option<Message>, send:Option<Message>)
 }
